DumbContracts/Proofs/SafeCounter/Basic.lean
@@ -94,11 +94,14 @@ theorem increment_meets_spec (s : ContractState)
   increment_spec s s' := by
   rw [increment_unfold s h_no_overflow]
   simp only [ContractResult.snd, increment_spec]
-  refine ⟨?_, ?_, trivial, trivial, trivial, trivial, trivial, trivial⟩
+  refine ⟨?_, ?_, ?_, ?_, ?_⟩
   · simp [evm_add_eq_of_no_overflow (s.storage 0) 1 h_no_overflow]
-  intro slot h_ne
-  simp [beq_iff_eq]
-  intro h_eq; exact absurd h_eq h_ne
+  · intro slot h_ne
+    simp [beq_iff_eq]
+    intro h_eq; exact absurd h_eq h_ne
+  · rfl
+  · rfl
+  · exact ⟨rfl, ⟨rfl, ⟨rfl, rfl⟩⟩⟩
 
 theorem increment_adds_one (s : ContractState)
   (h_no_overflow : (s.storage 0 : Nat) + 1 ≤ MAX_UINT256) :
@@ -150,11 +153,14 @@ theorem decrement_meets_spec (s : ContractState)
   decrement_spec s s' := by
   rw [decrement_unfold s h_no_underflow]
   simp only [ContractResult.snd, decrement_spec]
-  refine ⟨?_, ?_, trivial, trivial, trivial, trivial, trivial, trivial⟩
+  refine ⟨?_, ?_, ?_, ?_, ?_⟩
   · simp [HSub.hSub, sub]
-  intro slot h_ne
-  simp [beq_iff_eq]
-  intro h_eq; exact absurd h_eq h_ne
+  · intro slot h_ne
+    simp [beq_iff_eq]
+    intro h_eq; exact absurd h_eq h_ne
+  · rfl
+  · rfl
+  · exact ⟨rfl, ⟨rfl, ⟨rfl, rfl⟩⟩⟩
 
 theorem decrement_subtracts_one (s : ContractState)
   (h_no_underflow : (s.storage 0 : Nat) ≥ 1) :
